naive version

problems/5/Problem5.dfy
@@ -10,18 +10,26 @@ module Problem5 {
     function abs(x: int): nat {
         if x < 0 then -x else x
     }
-
-    // function rangeMapper(range: seq<seq<nat>>): nat -> nat 
-    //     requires forall x:: x in range ==> |x| == 3 
-    //     // ensures forall x:nat :: rangeMapper(range).requires(x)
-    // {
-    //     (x: nat) => if |range| == 0 then x else if range[0][1] <= x < range[0][1]+range[0][2] then range[0][0]+(x-range[0][1]) else rangeMapper(range[1..])(x)
-    // }
-    function rangeMapper(range: seq<seq<nat>>): nat -> nat 
-        (z: nat) => z
+    function min(a: nat ,b:nat): nat {
+        if a < b then a else b
     }
 
-    method parseInput(input:string) returns (seeds: seq<nat>, maps: seq<nat --> nat>) {
+    function rangeMapper(range: seq<seq<nat>>): nat -> nat 
+        requires forall x:: x in range ==> |x| == 3 
+        ensures forall x:nat :: rangeMapper(range).requires(x)
+    {
+        (x: nat) => if |range| == 0 then 
+            x 
+        else if range[0][1] <= x < range[0][1]+range[0][2] then 
+            range[0][0]+(x-range[0][1])
+        else 
+            rangeMapper(range[1..])(x)
+    }
+    // function rangeMapper(range: seq<seq<nat>>): nat -> nat {
+    //     (z: nat) => z
+    // }
+
+    method parseInput(input:string) returns (seeds: seq<nat>, maps: seq<nat -> nat>) {
         maps :=[];
         seeds := [];
         var sectionStrings := splitOnDoubleBreak(input);
@@ -48,19 +56,72 @@ module Problem5 {
         }
     }
 
+    method parseInput2(input:string) returns (seeds: seq<(nat, nat)>, maps: seq<nat -> nat>) {
+        maps :=[];
+        seeds := [];
+        var sectionStrings := splitOnDoubleBreak(input);
+        assume {:axiom} |sectionStrings| == 8;
+        expect |sectionStrings| == 8;
+        assume {:axiom} |sectionStrings[0]| > 6;
+        expect |sectionStrings[0]| > 6;
+        var seedString := sectionStrings[0][7..];
+        var seedsseq := Map(x => abs(Integer(x)), split(seedString, " "));
+        for i := 0 to |seedsseq|/2 {
+            seeds := seeds + [(seedsseq[2*i], seedsseq[2*i+1])];
+        }
+        print seeds, "\n";
+        for i:=1 to |sectionStrings| {
+            assume {:axiom} |splitOnBreak(sectionStrings[i])| > 0;
+            expect |splitOnBreak(sectionStrings[i])| > 0;
+            var mapString := splitOnBreak(sectionStrings[i])[1..];
+            var sections : seq<seq<nat>> := [];
+            for k := 0 to |mapString| {
+                if mapString[k] != "" {
+                    sections := sections + [Map(x => abs(Integer(x)), split(mapString[k], " "))];
+                }
+            }
+            print sections, "\n";
+            assume {:axiom} forall x :: x in sections ==> |x| == 3;
+            maps := maps + [rangeMapper(sections)];
+        }
+    }
+
+
     method problem5_1(input: string) returns (x: int) {
         var seeds, functs := parseInput(input);
+        assume {:axiom} |functs| > 1;
         print "\n", functs[0](48);
+        print "\n", "GOTHERE?";
         // print "\n", maps[0](51);
         // print "\n", maps[0](97);
         // print "\n", maps[0](98);
         // print "\n", maps[0](99);
-        var locations := Map((seed: nat) => FoldLeft((x: nat, f: nat -> nat) => f(x), seed, maps), seeds)
-        print locations;
-        return 3;
+        var locations := Map((seed: nat) => FoldLeft((x: nat, f: nat -> nat) => f(x), seed, functs), seeds);
+        print locations, "\nresult: ";
+        assume {:axiom} |locations| > 0;
+        return FoldLeft(min, locations[0], locations);
     }
 
     method problem5_2(input: string) returns (x: int) {
-        return 4;
+        var seeds, functs := parseInput2(input);
+        var minLoc:Option<nat> := None;
+        for i := 0 to |seeds| {
+            print "\n i: ",i, " ", seeds[i];
+            for k: nat := seeds[i].0 to seeds[i].0+seeds[i].1 {
+                var loc: nat := FoldLeft((x: nat, f: nat -> nat) => f(x), k, functs);
+                match minLoc {
+                    case None => {
+                        minLoc := Some(loc);
+                    }
+                    case Some(minloc) => {
+                        if loc < minloc {
+                            minLoc := Some(loc);
+                        }
+                    }
+                }
+            }
+        }
+        print "\n";
+        return minLoc.UnwrapOr(0);
     }
 }
